src/impl/TLS13.Impl.Server.Driver.Network.fst
@@ -8,6 +8,7 @@ open Pulse.Lib.Array.PtsTo
 module B = TLS13.Bytes
 module A = Pulse.Lib.Array
 module CL = TLS13.ConnectionLog
+module CPI = Common.ProtocolImplementation
 module CS = TLS13.Spec.StateMachine
 module CSL = TLS13.ConnectionState.Lemmas
 module CT = TLS13.Impl.Client.Types
@@ -17,10 +18,12 @@ module CQ = TLS13.Impl.ConnectionState.Queries
 module ID = FStar.IndefiniteDescription
 module IO = Common.TCP
 module M = TLS13.Messages
+module MR = Pulse.Lib.MonotonicGhostRef
 module R = Pulse.Lib.Reference
 module Seq = FStar.Seq
 module SeqP = FStar.Seq.Properties
 module S = TLS13.Impl.Server
+module SP = TLS13.Impl.Server.CanonicalProtocol
 module SZ = FStar.SizeT
 module ST = TLS13.Impl.Server.Types
 module T = TLS13.Types
@@ -1612,6 +1615,25 @@ fn process_buffered_network_bytes_compact_once
   assert (pure (SZ.v buffer_resp.ST.consumed_len <= B.length raw_prefix));
   assert (pure (SZ.v buffer_resp.ST.consumed_len <= SZ.v current_len));
   assert (pure (SZ.v buffer_resp.ST.consumed_len <= SZ.v buffered_len));
+  assert (pure (CPI.buffers_wf
+    raw_prefix
+    current_len
+    network_out
+    driver_network_out_capacity));
+  unfold (server_driver_canonical_progress d 'st0);
+  SP.lemma_server_network_event_progress
+    (Ghost.reveal d.server_driver_initial)
+    'st0
+    st1
+    buffer_resp
+    raw_prefix
+    current_len
+    network_out
+    network_out_bytes
+    driver_network_out_capacity
+    app_out_bytes;
+  MR.update d.server_driver_progress st1;
+  fold (server_driver_canonical_progress d st1);
 
   A.to_mask raw_prefix_array;
   with raw_prefix_mask_after.
